ulib/LowStar.Native.DynamicRegion.fsti
@@ -1,0 +1,216 @@
+(*
+   Copyright 2008-2019 Microsoft Research
+
+     Licensed under the Apache License, Version 2.0 (the "License");
+     you may not use this file except in compliance with the License.
+     You may obtain a copy of the License at
+
+         http://www.apache.org/licenses/LICENSE-2.0
+
+     Unless required by applicable law or agreed to in writing, software
+     distributed under the License is distributed on an "AS IS" BASIS,
+     WITHOUT WARRANTIES OR CONDITIONS OF ANY KIND, either express or implied.
+     See the License for the specific language governing permissions and
+     limitations under the License.
+*)
+module LowStar.Native.DynamicRegion
+open FStar.Preorder
+module U32 = FStar.UInt32
+module B = LowStar.Buffer
+module HS = FStar.HyperStack
+module HST = FStar.HyperStack.ST
+
+/// A dynamic region is a refinement of the regions defined in
+/// FStar.HyperStack (HS). Wheres HS regions are a purely static
+/// concept (they serve only to group related stack or heap references
+/// into an abstract footprint), dynamic regions allow concretely
+/// allocating heap references within a single abstract store and for
+/// that store to be reclaimed in bulk with a single operation to free
+/// the entire region.
+///
+/// This is beneficial for two reasons:
+///
+///  - The liveness of a references can be bound to the liveness of
+///    the region, so a client need only maintain the liveness of the
+///    region as an invariant, rather than the liveness of several
+///    (potentially unbounded) references.q
+/// 
+///  - This simplifies their concrete memory reclamation strategy and
+///    helps eliminate memory leaks
+///
+/// Not all references in a dynamic region need to be reclaimed in
+/// bulk. Some of them can be reclaimed early---for these, there is
+/// little additional benefit provided by this module over
+/// HS.rid. Still, we support such references for uniformity---a
+/// client can allocate a single drgn for both kinds of references,
+/// rather than needing to allocate a separate rid for short-lived
+/// allocations. In the future, the runtime support for this library
+/// will also support reclaiming when the region is freed all
+/// short-lived references that have not yet been explicitly
+/// freed. However, for now, any such short-lived reference must be
+/// free explicitly to avoid a memory leak.
+///
+/// In addition to references, this module supports allocating and
+/// freeing buffers within dynamic regions, again in two varieties:
+/// region lifetime and early frees.
+///
+/// Dynamic regions resemble constructs in other languages, notably
+/// support for Berger et al.'s "reaps" in Cyclone
+///
+///   https://people.cs.umass.edu/~emery/pubs/berger-oopsla2002.pdf
+///   http://www.cs.umd.edu/projects/PL/cyclone/scp.pdf
+
+
+/// We distinguish heap regions from stack regions
+/// Dynamic regions are for the heap only
+let is_heap_region (r:HS.rid) : GTot bool =
+  HS.is_eternal_color (HS.color r) //we should rename HS.is_eternal_region to HS.is_heap_region
+
+/// All eternal regions are heap_regions
+let eternal_heap_regions (r:HS.rid) 
+  : Lemma (HST.is_eternal_region r ==> is_heap_region r)
+  = ()
+
+/// The type of heap regions
+let h_rid = r:HS.rid { is_heap_region r }
+
+/// A wrapper around a library function to create a new heap region
+let new_heap_region (m:HS.mem) 
+                    (parent:h_rid{HS.live_region m parent})
+  : Tot (t:(h_rid * HS.mem){HS.fresh_region (fst t) m (snd t)})
+  = let rid, m = HS.new_eternal_region m parent None in
+    rid, m
+
+/// At runtime, this is extracted to the `handle`
+/// type from LowStar.RegionAllocator
+val drgn : Type0
+
+/// The model provides a way to project a classic "static"
+/// heap region identifier from a drgn
+val rid_of_drgn: drgn -> Tot h_rid
+
+/// Allocates a fresh dynamic region within parent
+/// Spec is similar to ST.new_region
+/// Extracted to `new_handle`
+val new_drgn (parent:HST.erid)
+  : HST.ST drgn
+    (requires fun m        -> True)
+    (ensures  fun m0 d m1 ->
+      let r0 = parent in
+      let r1 = rid_of_drgn d in
+      let open HS in
+      r1 `extends` r0 /\
+      fresh_region r1 m0 m1 /\
+      color r1 = color r0 /\
+      get_hmap m1 == Map.upd (get_hmap m0) r1 Heap.emp /\
+      get_tip m1 == get_tip m0 /\ 
+      live_region m0 r0 /\
+      (r1, m1) == new_heap_region m0 r0)
+
+/// Deallocates the region and all its contained objects
+/// (Similar in spirit to pop_frame)
+/// Exracted to `free_handle`
+val free_drgn (d:drgn)
+  : HST.ST unit
+    (requires fun h -> 
+      HS.live_region h (rid_of_drgn d))
+    (ensures fun h0 _ h1 -> 
+      B.modifies (B.loc_region_only false (rid_of_drgn d)) h0 h1)
+
+(*** Allocating and Free'ing references ***)
+
+/// We support allocating two kinds of references in a dynamic region:
+///
+///   -- region-lifetime refs are live so long as their enclosing
+///      region is live. They are reclaimed only when the entire
+///      region is reclaimed
+/// 
+///   -- short-lived refs are associated with the region, but they can
+///      be allocated and freed manually
+
+
+/// This is an abstract predicate recording that `r`'s lifetime is
+/// bound to the lifetime of `d`
+val region_lifetime_ref (#a:Type) (#rel:preorder a) (d:drgn) (r:HST.mref a rel) : prop
+
+/// Eliminating the abstract predicate via a stateful lemma, i.e., a "recall"
+val recall_liveness_ref (#a:Type) (#rel:preorder a) (d:drgn) (r:HST.mref a rel) 
+  : HST.ST unit
+    (requires fun h ->
+      region_lifetime_ref d r /\
+      HS.live_region h (rid_of_drgn d))
+    (ensures fun h0 _ h1 ->
+      h0 == h1 /\
+      h1 `HS.contains` r)
+
+/// Allocate a "region-lifetime" reference to `init` in
+/// within `d`. The returned reference is live so long as `d` is
+/// Extracted to `a *p = (a)RegionAllocator.alloc d (sizeof a); *p = init;`
+val ralloc (#a:Type) (#rel:preorder a) (d:drgn) (init:a)
+  : HST.ST (HST.mref a rel)
+    (requires fun h ->
+      HS.live_region h (rid_of_drgn d))
+    (ensures fun h0 r h1 -> 
+      HST.ralloc_post (rid_of_drgn d) init h0 r h1 /\
+      region_lifetime_ref d r)
+  
+/// Allocate a manually-managed reference to `init` within `d`.
+/// Extracted as just a normal `malloc` (not allocated concretely in d)
+///
+/// Note: this could almost be implemented directly using HST.ralloc_mm
+/// 
+/// However, that function is specialized to work only on HST.is_eternal_region
+/// That restriction should be relaxed
+val ralloc_mm (#a:Type) (#rel:preorder a) (d:drgn) (init:a)
+  : HST.ST (HST.mmmref a rel)
+    (requires fun h ->
+      HS.live_region h (rid_of_drgn d))
+    (ensures fun h0 r h1 -> 
+      HST.ralloc_post (rid_of_drgn d) init h0 r h1)
+
+/// Free a manually-managed reference
+/// Extracted as just an normal `free` (since r is not allocated concretely in d)
+inline_for_extraction
+let rfree (#a:Type) (#rel:preorder a) (r:HST.mmmref a rel)
+  : HST.ST unit
+    (requires fun h -> 
+      h `HS.contains` r)
+    (ensures fun h0 _ h1 -> 
+      B.modifies (B.loc_freed_mreference r) h0 h1)
+  = HST.rfree r
+
+(*** Allocating and Free'ing buffers ***)
+
+/// This is an abstract predicate recording that the buffer `b`'s lifetime is
+/// bound to the lifetime of `d`
+val region_lifetime_buf (#a:Type) (#rrel #rel:B.srel a) (d:drgn) (b:B.mbuffer a rrel rel) : prop
+
+/// Eliminating the abstract predicate via a stateful lemma, i.e., a "recall"
+val recall_liveness_buf (#a:Type) (#rrel #rel:B.srel a) (d:drgn) (b:B.mbuffer a rrel rel)
+  : HST.ST unit
+    (requires fun h ->
+      region_lifetime_buf d b /\
+      HS.live_region h (rid_of_drgn d))
+    (ensures fun h0 _ h1 ->
+      h0 == h1 /\
+      h1 `B.live` b)
+
+/// Allocating a region-lifetime buffer
+val ralloc_buf (#a:Type0) (#rrel:B.srel a) (r:drgn) (init:a) (len:U32.t)
+  : HST.ST (B.lmbuffer a rrel rrel (U32.v len))
+    (requires fun h ->
+      U32.v len > 0 /\
+      HS.live_region h (rid_of_drgn r))
+    (ensures fun h0 b h1 ->
+      B.alloc_post_mem_common b h0 h1 (Seq.create (U32.v len) init) /\
+      region_lifetime_buf r b)
+
+/// Allocating a buffer that can be freed early
+val ralloc_mm_buf (#a:Type0) (#rrel:B.srel a) (r:drgn) (init:a) (len:U32.t)
+  : HST.ST (B.lmbuffer a rrel rrel (U32.v len))
+    (requires fun h ->
+      U32.v len > 0 /\
+      HS.live_region h (rid_of_drgn r))
+    (ensures fun h0 b h1 ->
+      B.alloc_post_mem_common b h0 h1 (Seq.create (U32.v len) init))
+
